theories/SpecNotations.v
@@ -1,12 +1,31 @@
 Require Import Blech.Spec.
 
+Require Import Coq.Unicode.Utf8.
+
 Bind Scope list_scope with environment.
 Bind Scope list_scope with subst.
 Bind Scope list_scope with usage.
+Bind Scope list_scope with sorts.
+Bind Scope list_scope with functions.
+Bind Scope list_scope with relations.
+Bind Scope list_scope with theory.
 
 Infix "*" := t_prod.
 
 Notation "'η'" := (eta) (at level 0).
+
+Definition eq_usage (Δ Δ': usage): {Δ = Δ'} + {Δ ≠ Δ'}.
+Proof.
+  decide equality.
+  destruct a as [x u], p as [y u'].
+  destruct (eq_var x y), (eq_use u u').
+  all: subst.
+  all: auto.
+  all: right.
+  all: intro p.
+  all: inversion p.
+  all: auto.
+Defined.
 
 (* Notation "( X , F , G ) ⊢ v ⇐ t" := (Jv X F G v t) (at level 90). *)
 (* Notation "( X , F , G ) ⊢ V ⇒ t" := (JV X F G V t) (at level 90). *)
