theories/Theory.v
@@ -1,0 +1,86 @@
+Require Import Blech.Spec.
+Require Import Blech.SpecNotations.
+Require Blech.Term.
+Require Blech.Context.
+
+Require Import Coq.Unicode.Utf8.
+Require Coq.Lists.List.
+
+Import List.ListNotations.
+Import IfNotations.
+
+Require Import FunInd.
+
+Implicit Type Γ: environment.
+Implicit Type Δ: usage.
+Implicit Type E: context.
+Implicit Type τ: type.
+Implicit Types x y: var.
+Implicit Type ρ: subst.
+Implicit Type v: intro.
+
+Definition check_sequent (S: sorts) (F: functions) (R: relations) (H: sequent): bool :=
+  match H with
+  | H_seq Γ c c' =>
+      let all := useall Γ in
+      let none := usenone Γ in
+      Context.typeinfer S F R Γ c
+      && (if Context.useinfer none c is Some Δ then if eq_usage Δ all then true else false else false)
+      && Context.typeinfer S F R Γ c'
+      && (if Context.useinfer none c' is Some Δ then if eq_usage Δ all then true else false else false)
+  end %bool.
+
+Function check_theory (S: sorts) (F: functions) (R: relations) (T: theory): bool :=
+  if T is cons H T' then
+    andb (check_sequent S F R H) (check_theory S F R T')
+  else
+    true.
+
+Lemma check_sequent_sound {S F R H}: Bool.Is_true (check_sequent S F R H) → JH S F R H.
+Proof.
+  destruct H.
+  cbn.
+  intros p.
+  destruct
+    Context.typeinfer eqn:q1,
+    Context.useinfer eqn:q2.
+  all: try contradiction.
+  destruct eq_usage in p.
+  2: contradiction.
+  subst.
+  cbn in p.
+  destruct Context.typeinfer eqn:q3 in p.
+  2: contradiction.
+  destruct Context.useinfer eqn:q4 in p.
+  2: contradiction.
+  destruct eq_usage in p.
+  2: contradiction.
+  subst.
+  constructor.
+  - apply Context.typeinfer_sound.
+    rewrite q1.
+    constructor.
+  - apply Context.typeinfer_sound.
+    rewrite q3.
+    constructor.
+  - apply Context.useinfer_sound.
+    eauto.
+  - apply Context.useinfer_sound.
+    auto.
+Qed.
+
+Lemma check_theory_sound {S F R T}: Bool.Is_true (check_theory S F R T) → JT S F R T.
+Proof.
+  functional induction (check_theory S F R T).
+  all: intros.
+  - destruct check_sequent eqn:q1.
+    2: contradiction.
+    constructor.
+    + apply check_sequent_sound.
+      rewrite q1.
+      constructor.
+    + eauto.
+  - destruct T.
+    2: contradiction.
+    constructor.
+Qed.
